Almost finish the dead_calls proof

proofs/compiler/dead_calls_proof.v
@@ -73,11 +73,23 @@ Definition CallsE :=
    i_Calls_call, c_Calls_nil , c_Calls_cons ).
 
 (* -------------------------------------------------------------------- *)
-Lemma i_callsE c i : i_calls c i = Sp.union c (i_Calls i).
-Proof. Admitted.
-
-Lemma c_callsE c i : c_calls c i = Sp.union c (c_Calls i).
-Proof. Admitted.
+Lemma c_callsE c i : Sp.Equal (c_calls c i) (Sp.union c (c_Calls i)).
+Proof.
+move: c.
+apply (@cmd_rect
+         (fun i => forall c, Sp.Equal (i_calls_r c i) (Sp.union c (i_Calls_r i)))
+         (fun i => forall c, Sp.Equal (i_calls c i) (Sp.union c (i_Calls i)))
+         (fun i => forall c, Sp.Equal (c_calls c i) (Sp.union c (c_Calls i)))) => /=
+  [ i0 ii Hi | | i0 c0 Hi Hc | x t e | xs o es | e c1 c2 Hc1 Hc2
+    | v dir lo hi c0 Hc | c0 e c' Hc Hc' | ii xs f es] c //.
++ rewrite CallsE; SpD.fsetdec.
++ rewrite /= CallsE Hc Hi; SpD.fsetdec.
++ SpD.fsetdec.
++ SpD.fsetdec.
++ rewrite -/(foldl _ _) -/(foldl _ _) -/(c_calls _ _) -/(c_calls _ _) Hc2 Hc1 -/(c_Calls _) -/(c_Calls _); SpD.fsetdec.
++ rewrite -/(foldl _ _) -/(foldl _ _) -/(c_calls _ _) -/(c_calls _ _) Hc' Hc -/(c_Calls _) -/(c_Calls _); SpD.fsetdec.
++ SpD.fsetdec.
+Qed.
 
 (* -------------------------------------------------------------------- *)
 Lemma dead_calls_subseq c p : subseq (dead_calls c p) p.
@@ -86,7 +98,7 @@ elim: p c => [|[f fd] p ih] c //=; case: ifPn => _; last first.
 + case E: (dead_calls _ _) => [//|[f' fd'] p'].
   case: ifPn => _; last by rewrite -E. have := ih c.
   by rewrite E => /(subseq_trans _); apply; apply/subseq_cons.
-by rewrite eqxx c_callsE; apply: ih.
+rewrite eqxx; exact: ih.
 Qed.
 
 (* -------------------------------------------------------------------- *)
@@ -112,7 +124,276 @@ Definition pg_compat_call :=
     sem_call p' m f args m' res.
 End PgCompat.
 
+Lemma subseq_in {T: eqType} (s: seq T) s' x: subseq s s' -> x \in s -> x \in s'.
+Proof.
+elim: s' s=> [|a' l' IH] s //=.
++ by move=> /eqP ->.
+move: s IH=> [] // a l IH.
+case: ifP.
++ move=> /eqP -> Hsub // H.
+  rewrite in_cons in H.
+  move: H=> /orP; case.
+  + move=> /eqP ->.
+    exact: mem_head.
+  + move=> /(IH _ Hsub) H.
+    by rewrite in_cons H orbT.
+move=> _ Hsub Hin.
+have H := IH _ Hsub Hin.
+by rewrite in_cons H orbT.
+Qed.
+
+Lemma get_same (p p': prog) fn fd fd':
+  uniq (map fst p) ->
+  subseq p' p ->
+  get_fundef p fn = Some fd ->
+  get_fundef p' fn = Some fd' ->
+  fd = fd'.
+Proof.
+  elim: p p'=> [] // -[fn0 fd0] l IH /= p' /andP [Hnot Huniq].
+  case: p' IH=> [] // [fn1 fd1] l1 IH.
+  case: ifP.
+  + move=> /eqP ->.
+    rewrite !get_fundef_cons /=.
+    case: ifP.
+    + by move=> _ _ []<- []<-.
+    move=> _ Hsub H0 H1.
+    exact: (IH _ _ Hsub).
+  move=> Hdiff Hsub.
+  move: Hdiff=> /eqP Hdiff.
+  rewrite !get_fundef_cons /=.
+  case: ifP.
+  + move=> /eqP? []?; subst fn fd.
+    move=> H.
+    exfalso; move: Hnot=> /negP; apply.
+    apply: subseq_in.
+    apply: map_subseq Hsub.
+    case: ifP H.
+    + move=> /eqP?[]?; subst fn1 fd1.
+      by rewrite /= in_cons eq_refl.
+    move=> _ Hget.
+    have Hin := get_fundef_in Hget.
+    by rewrite in_cons /= Hin orbT.
+  move=> _ H.
+  case: ifP.
+  + move=> /eqP? []?; subst fn fd'.
+    apply: (IH _ _ Hsub)=> //.
+    by rewrite get_fundef_cons /= eq_refl.
+  move=> Hneq H1.
+  apply: (IH _ _ Hsub H)=> //.
+  by rewrite get_fundef_cons /= Hneq.
+Qed.
+
+Lemma get_dead_calls p fn f f0:
+  Sp.In fn f ->
+  get_fundef p fn = Some f0 ->
+  get_fundef (dead_calls f p) fn = Some f0.
+Proof.
+  elim: p f=> [] // -[fn0 fd0] l IH /= f Hin.
+  rewrite get_fundef_cons /=.
+  case: ifP.
+  + move=> /eqP?[]?; subst fn0 f0.
+    move: Hin=> /SpD.F.mem_1 ->.
+    by rewrite get_fundef_cons /= eq_refl.
+  move=> Hneq H.
+  have Hin': Sp.In fn (c_calls f (f_body fd0)).
+    rewrite c_callsE; SpD.fsetdec.
+  case: ifP.
+  + move=> ?.
+    rewrite get_fundef_cons /= Hneq.
+    exact: IH.
+  move=> _; exact: IH.
+Qed.
+
+Section PROOF.
+  Variables (f : Sp.t) (p: prog).
+  Hypothesis p_uniq: uniq (map fst p).
+  Definition p' := dead_calls f p.
+
+  Definition def_incl sv :=
+    forall x : positive, Sp.In x sv -> exists fd, get_fundef p' x = Some fd.
+
+  Lemma call_stbl fn fd:
+    get_fundef p' fn = Some fd -> def_incl (c_Calls fd.(f_body)).
+  Proof.
+  Admitted.
+
+  Lemma def_incl_union a b:
+    def_incl (Sp.union a b) -> def_incl a /\ def_incl b.
+  Proof.
+    split=> x Hx; apply: H; SpD.fsetdec.
+  Qed.
+
+  Let Pi (s:estate) (i:instr) (s':estate) :=
+    def_incl (i_Calls i) -> sem_I p s i s' -> sem_I p' s i s'.
+
+  Let Pi_r (s:estate) (i:instr_r) (s':estate) :=
+    def_incl (i_Calls_r i) -> sem_i p s i s' -> sem_i p' s i s'.
+
+  Let Pc (s:estate) (c:cmd) (s':estate) :=
+    def_incl (c_Calls c) -> sem p s c s' -> sem p' s c s'.
+
+  Let Pfor (i:var_i) vs s c s' :=
+    def_incl (c_Calls c) -> sem_for p i vs s c s' -> sem_for p' i vs s c s'.
+
+  Let Pfun m1 fn vargs m2 vres :=
+    def_incl (Sp.singleton fn) -> sem_call p m1 fn vargs m2 vres -> sem_call p' m1 fn vargs m2 vres.
+
+  Local Lemma Hskip s : Pc s [::] s.
+  Proof. move=> _ _; exact: Eskip. Qed.
+
+  Local Lemma Hcons s1 s2 s3 i c :
+    sem_I p s1 i s2 ->
+    Pi s1 i s2 -> sem p s2 c s3 -> Pc s2 c s3 -> Pc s1 (i :: c) s3.
+  Proof.
+    move=> Hsi Hi Hsc Hc Hincl.
+    rewrite CallsE in Hincl.
+    move: Hincl=> /def_incl_union [Hincli Hinclc] H.
+    exact: (Eseq (Hi Hincli Hsi) (Hc Hinclc Hsc)).
+  Qed.
+
+  Local Lemma HmkI ii i s1 s2 :
+    sem_i p s1 i s2 -> Pi_r s1 i s2 -> Pi s1 (MkI ii i) s2.
+  Proof.
+    move=> Hs Hi Hincl _.
+    apply: EmkI.
+    exact: (Hi Hincl Hs).
+  Qed.
+
+  Local Lemma Hassgn s1 s2 l tag e :
+    Let v := sem_pexpr s1 e in write_lval l v s1 = Ok error s2 ->
+    Pi_r s1 (Cassgn l tag e) s2.
+  Proof.
+    move=> H _ _; exact: (Eassgn _ _ H).
+  Qed.
+
+  Local Lemma Hopn s1 s2 o xs es :
+    Let x := Let x := sem_pexprs s1 es in sem_sopn o x
+    in write_lvals s1 xs x = Ok error s2 -> Pi_r s1 (Copn xs o es) s2.
+  Proof.
+    move=> H _ _; exact: (Eopn _ H).
+  Qed.
+
+  Local Lemma Hif_true s1 s2 e c1 c2 :
+    Let x := sem_pexpr s1 e in to_bool x = Ok error true ->
+    sem p s1 c1 s2 -> Pc s1 c1 s2 -> Pi_r s1 (Cif e c1 c2) s2.
+  Proof.
+    move=> H Hsi Hc Hincl _.
+    rewrite CallsE in Hincl.
+    move: Hincl=> /def_incl_union [Hincl1 Hincl2].
+    apply: (Eif_true _ H).
+    exact: (Hc Hincl1 Hsi).
+  Qed.
+
+  Local Lemma Hif_false s1 s2 e c1 c2 :
+    Let x := sem_pexpr s1 e in to_bool x = Ok error false ->
+    sem p s1 c2 s2 -> Pc s1 c2 s2 -> Pi_r s1 (Cif e c1 c2) s2.
+  Proof.
+    move=> H Hsi Hc Hincl _.
+    rewrite CallsE in Hincl.
+    move: Hincl=> /def_incl_union [Hincl1 Hincl2].
+    apply: (Eif_false _ H).
+    exact: (Hc Hincl2 Hsi).
+  Qed.
+
+  Local Lemma Hwhile_true s1 s2 s3 s4 c e c' :
+    sem p s1 c s2 -> Pc s1 c s2 ->
+    Let x := sem_pexpr s2 e in to_bool x = ok true ->
+    sem p s2 c' s3 -> Pc s2 c' s3 ->
+    sem_i p s3 (Cwhile c e c') s4 -> Pi_r s3 (Cwhile c e c') s4 -> Pi_r s1 (Cwhile c e c') s4.
+  Proof.
+    move=> Hs1 Hc1 H Hs2 Hc2 Hsw Hiw Hinclw _.
+    rewrite CallsE in Hinclw.
+    have /def_incl_union [Hincl Hincl'] := Hinclw.
+    exact: (Ewhile_true (Hc1 Hincl Hs1) H (Hc2 Hincl' Hs2) (Hiw Hinclw Hsw)).
+  Qed.
+
+  Local Lemma Hwhile_false s1 s2 c e c' :
+    sem p s1 c s2 -> Pc s1 c s2 ->
+    Let x := sem_pexpr s2 e in to_bool x = ok false ->
+    Pi_r s1 (Cwhile c e c') s2.
+  Proof.
+    move=> Hs1 Hc1 H Hinclw _.
+    rewrite CallsE in Hinclw.
+    have /def_incl_union [Hincl Hincl'] := Hinclw.
+    exact: (Ewhile_false _ (Hc1 Hincl Hs1) H).
+  Qed.
+
+  Local Lemma Hfor s1 s2 (i:var_i) d lo hi c vlo vhi :
+    Let x := sem_pexpr s1 lo in to_int x = Ok error vlo ->
+    Let x := sem_pexpr s1 hi in to_int x = Ok error vhi ->
+    sem_for p i (wrange d vlo vhi) s1 c s2 ->
+    Pfor i (wrange d vlo vhi) s1 c s2 -> Pi_r s1 (Cfor i (d, lo, hi) c) s2.
+  Proof.
+    move=> Hlo Hhi Hsf Hf Hincl _.
+    rewrite CallsE in Hincl.
+    apply: (Efor Hlo Hhi).
+    exact: (Hf Hincl Hsf).
+  Qed.
+
+  Local Lemma Hfor_nil s i c: Pfor i [::] s c s.
+  Proof.
+    move=> Hincl _; exact: EForDone.
+  Qed.
+
+  Local Lemma Hfor_cons s1 s1' s2 s3 (i : var_i) (w:Z) (ws:seq Z) c :
+    write_var i w s1 = Ok error s1' ->
+    sem p s1' c s2 ->
+    Pc s1' c s2 ->
+    sem_for p i ws s2 c s3 -> Pfor i ws s2 c s3 -> Pfor i (w :: ws) s1 c s3.
+  Proof.
+   move=> H Hsc Hc Hsf Hf Hincl _.
+   exact: (EForOne H (Hc Hincl Hsc) (Hf Hincl Hsf)).
+  Qed.
+
+  Local Lemma Hcall s1 m2 s2 ii xs fn args vargs vs:
+    sem_pexprs s1 args = Ok error vargs ->
+    sem_call p (emem s1) fn vargs m2 vs ->
+    Pfun (emem s1) fn vargs m2 vs ->
+    write_lvals {| emem := m2; evm := evm s1 |} xs vs = Ok error s2 ->
+    Pi_r s1 (Ccall ii xs fn args) s2.
+  Proof.
+    move=> Hargs Hcall Hfun Hres Hincl Hsi.
+    apply: (Ecall _ Hargs _ Hres).
+    exact: Hfun.
+  Qed.
+
+  Local Lemma Hproc m1 m2 fn fd vargs s1 vm2 vres:
+    get_fundef p fn = Some fd ->
+    write_vars (f_params fd) vargs {| emem := m1; evm := vmap0 |} = ok s1 ->
+    sem p s1 (f_body fd) {| emem := m2; evm := vm2 |} ->
+    Pc s1 (f_body fd) {| emem := m2; evm := vm2 |} ->
+    mapM (fun x : var_i => get_var vm2 x) (f_res fd) = ok vres ->
+    List.Forall is_full_array vres ->
+    Pfun m1 fn vargs m2 vres.
+  Proof.
+    move=> Hget Hvargs Hsem Hc Hvres Hfull Hin Hcall.
+    have [|fd' Hfd'] := Hin fn; first by SpD.fsetdec.
+    have H := (get_same p_uniq (dead_calls_subseq f p) Hget Hfd'); subst fd'.
+    apply: (EcallRun _ Hvargs _ Hvres Hfull)=> //.
+    apply: Hc=> //.
+    apply: (call_stbl Hfd').
+  Qed.
+
+  Lemma dead_calls_callP fd mem mem' va vr:
+    Sp.In fd f ->
+    sem_call p mem fd va mem' vr ->
+    sem_call p' mem fd va mem' vr.
+  Proof.
+    move=> Hincl H.
+    apply: (@sem_call_Ind p Pc Pi_r Pi Pfor Pfun Hskip Hcons HmkI Hassgn Hopn
+             Hif_true Hif_false Hwhile_true Hwhile_false Hfor Hfor_nil Hfor_cons Hcall Hproc)=> //.
+    sinversion H.
+    move=> {H1 H2 H3 H4} x Hx.
+    have ? : x = fd by SpD.fsetdec.
+    subst x=> {Hx}.
+    exists f0.
+    rewrite /p'.
+    exact: get_dead_calls.
+  Qed.
+End PROOF.
+
 (* -------------------------------------------------------------------- *)
+(*
 Lemma pg_compat_sub c1 c2 p p' : Sp.Subset c2 c1 ->
      pg_compat_call c1 p p'
   -> pg_compat_call c2 p p'.
@@ -162,6 +443,19 @@ Local Hint Resolve pg_compat_for_body.
 Local Hint Constructors sem sem_I sem_i sem_for sem_call.
 
 (* -------------------------------------------------------------------- *)
+Lemma __ok p m f args m' res fd p' :
+     pg_compat_call (c_Calls fd.(f_body)) p p'
+  -> sem_call ((f, fd) :: p ) m f args m' res
+  -> sem_call ((f, fd) :: p') m f args m' res.
+Proof.
+move=> Hcompat Hcall.
+sinversion Hcall.
+apply: (EcallRun _ H0 _ H2)=> //.
+rewrite get_fundef_cons /= eq_refl.
+by rewrite get_fundef_cons /= eq_refl in H.
+admit.
+Admitted.
+
 Lemma _ok p m f args m' res fd p' :
      pg_compat_call (c_Calls fd.(f_body)) p p'
   -> sem_call ((f, fd) :: p ) m f args m' res
@@ -185,15 +479,59 @@ pose PC m f args m' res :=
   -> sem_call ((f, fd) :: p') m f args m' res.
 apply: (@sem_call_Ind p Pc Pi PI Pf PC);
   rewrite {}/Pc {}/Pi {}/PI {}/Pf {}/PC; try by eauto 7.
-+ admit.
-+ admit.
++ move=> ?????????.
+  move=> Hargs Hcall _ Hres Hcompat Hi.
+  apply: (Ecall _ Hargs _ Hres).
+  apply: Hcompat=> //.
+  rewrite CallsE; SpD.fsetdec.
++ move=> ???????? Hget Hargs ? IH Hres ? Hcompat Hcall.
+  admit.
+  apply: EcallRun.
+  rewrite get_fundef_cons /= eq_refl //.
+  admit.
+  apply: (EcallRun _ Hargs _ Hres)=> //.
+  rewrite get_fundef_cons /= eq_refl.
 + admit.
 Admitted.
 
 (* -------------------------------------------------------------------- *)
 Lemma dead_calls_ok (f : Sp.t) (p : prog) : uniq (map fst p) ->
   pg_compat_call f p (dead_calls f p).
-Proof. Admitted.
+Proof.
+elim: p=> [|[fn fd] l IH] Huniq //=.
+case: ifP=> Hmem.
++ move=> m e args m' res e_in_f Hcall.
+  case/boolP: (e == fn)=> /eqP.
+  + move=> ?; subst e.
+    apply: (_ok _ Hcall).
+    admit. (* using IH *)
+  admit.
+move=> m e args m' res e_in_f Hcall.
+apply: IH=> //.
+admit.
+  have := _ok _ Hcall.
+  apply: _ok.
+Print dead_calls.
+*)
+
+Lemma foldl_compat x y l (x_eq_y: Sp.Equal x y):
+  Sp.Equal (foldl (fun f c => Sp.add c f) x l)
+           (foldl (fun f c => Sp.add c f) y l).
+Proof.
+elim: l x y x_eq_y=> // a l IH /= x y x_eq_y.
+by apply: IH; SpD.fsetdec.
+Qed.
+
+Lemma foldlE a l x:
+  Sp.Equal (foldl (fun f c => Sp.add c f) x (a :: l))
+           (Sp.add a (foldl (fun f c => Sp.add c f) x l)).
+Proof.
+elim: l a x=> // a0 l IH a x.
+rewrite /= in IH.
+rewrite /=.
+rewrite -IH.
+apply: foldl_compat; SpD.fsetdec.
+Qed.
 
 (* -------------------------------------------------------------------- *)
 Lemma dead_calls_errP (s : seq funname) (p p': prog) : 
@@ -201,5 +539,10 @@ Lemma dead_calls_errP (s : seq funname) (p p': prog) :
   forall f m args m' res, f \in s -> 
     sem_call p  m f args m' res ->
     sem_call p' m f args m' res.
-Proof. Admitted.
-
+Proof.
+rewrite /dead_calls_err; case: ifP=> // /negbFE H []<- f m args m' res fins Hcall.
+apply: dead_calls_callP=> //.
+elim: s fins=> // a l IH Hin.
+rewrite foldlE.
+rewrite in_cons in Hin; case/orP: Hin=> [/eqP ->|/IH Hin]; SpD.fsetdec.
+Qed.
